Examples.lean
@@ -7,6 +7,7 @@ import Examples.Language.Buffer
 import Examples.Language.BufferCompiled
 import Examples.Language.Factorial
 import Examples.Language.FactorialCompiled
+import Examples.Language.Imports
 import Examples.Language.Linking
 import Examples.Language.Remainder
 import Examples.Language.Scalar
